src/SelectionSort.thy
@@ -2,8 +2,8 @@ theory SelectionSort
   imports Main IO IOArray
 begin
 
-fun selection_sort :: "nat io_array \<Rightarrow> nat \<Rightarrow> unit io" where
-  "selection_sort arr n = forMu (map nat [1..int n]) (\<lambda>i. do {
+fun selection_sort :: "nat io_array \<Rightarrow> unit io" where
+  "selection_sort arr = (let n = get_size arr in forMu (map nat [1..int n]) (\<lambda>i. do {
     min_ref \<leftarrow> ref i;
     forMu (map nat [int i+1..int n]) (\<lambda>j. do {
       valJ \<leftarrow> read_array arr j;
@@ -14,9 +14,25 @@ fun selection_sort :: "nat io_array \<Rightarrow> nat \<Rightarrow> unit io" whe
     m \<leftarrow> ! min_ref;
     swap_array arr i m;
     return ()
-  })"
+  }))"
 
 export_code selection_sort in Haskell
   module_name SelectionSort file "gen/"
+
+primrec sorted :: "'a::ord list \<Rightarrow> bool" where
+  "sorted [] = True"
+| "sorted (x#xs) = ((\<forall>y\<in>set xs. x \<le> y) \<and> sorted xs)"
+
+fun selection_sort_program where
+  "selection_sort_program xs = do {
+    arr \<leftarrow> write_list_as_array xs;
+    selection_sort arr;
+    read_list_from_array arr
+  }"
+
+theorem selection_sort_is_sorted:
+  assumes "effect (run_io (selection_sort_program xs)) h h' rs"
+  shows "sorted rs"
+  sorry
 
 end
