src/IO.thy
@@ -28,39 +28,39 @@ lemma monad_assoc[simp]:
   shows "(m \<bind> f) \<bind> g = m \<bind> (\<lambda>x. f x \<bind> g)"
   unfolding bind_def comp_def by (auto split: prod.splits)
 
-definition present :: "heap \<Rightarrow> 'a::heap ref \<Rightarrow> bool" where
-  "present h r \<longleftrightarrow> addr_of_ref r < lim h"
+definition present_heap :: "heap \<Rightarrow> 'a::heap ref \<Rightarrow> bool" where
+  "present_heap h r \<longleftrightarrow> addr_of_ref r < lim h"
 
-definition get :: "heap \<Rightarrow> 'a::heap ref \<Rightarrow> 'a" where
-  "get h = from_nat \<circ> refs h TYPEREP('a) \<circ> addr_of_ref"
+definition get_heap :: "heap \<Rightarrow> 'a::heap ref \<Rightarrow> 'a" where
+  "get_heap h = from_nat \<circ> refs h TYPEREP('a) \<circ> addr_of_ref"
 
-definition set :: "'a::heap ref \<Rightarrow> 'a \<Rightarrow> heap \<Rightarrow> heap" where
-  "set r x = refs_update
+definition set_heap :: "'a::heap ref \<Rightarrow> 'a \<Rightarrow> heap \<Rightarrow> heap" where
+  "set_heap r x = refs_update
     (\<lambda>h. h(TYPEREP('a) := ((h (TYPEREP('a))) (addr_of_ref r := to_nat x))))"
 
-definition alloc :: "nat \<Rightarrow> heap \<Rightarrow> 'a::heap ref \<times> heap" where
-  "alloc s h = (let
+definition alloc_heap :: "nat \<Rightarrow> heap \<Rightarrow> 'a::heap ref \<times> heap" where
+  "alloc_heap s h = (let
      l = lim h;
      r = Ref l
    in (r, (h\<lparr>lim := l + s\<rparr>)))"
 
 definition new :: "'a \<Rightarrow> heap \<Rightarrow> 'a::heap ref \<times> heap" where
-  "new v h = (case alloc 1 h of (aref,h') \<Rightarrow> (aref, set aref v h'))"
+  "new v h = (case alloc_heap 1 h of (aref,h') \<Rightarrow> (aref, set_heap aref v h'))"
 
 definition noteq :: "'a::heap ref \<Rightarrow> 'b::heap ref \<Rightarrow> bool" (infix "=!=" 70) where
   "r =!= s \<longleftrightarrow> TYPEREP('a) \<noteq> TYPEREP('b) \<or> addr_of_ref r \<noteq> addr_of_ref s"
 
-definition allocate :: "nat \<Rightarrow> 'a::heap ref io" where
-  "allocate s = IO (Heap_Monad.heap (alloc s))"
+definition alloc :: "nat \<Rightarrow> 'a::heap ref io" where
+  "alloc s = IO (Heap_Monad.heap (alloc_heap s))"
 
 definition ref :: "'a::heap \<Rightarrow> 'a ref io" where
   [code del]: "ref v = IO (Heap_Monad.heap (new v))"
 
 definition lookup :: "'a::heap ref \<Rightarrow> 'a io" ("!_" 61) where
-  [code del]: "lookup r = IO (Heap_Monad.tap (\<lambda>h. get h r))"
+  [code del]: "lookup r = IO (Heap_Monad.tap (\<lambda>h. get_heap h r))"
 
 definition update :: "'a ref \<Rightarrow> 'a::heap \<Rightarrow> unit io" ("_ := _" 62) where
-  [code del]: "update r v = IO (Heap_Monad.heap (\<lambda>h. ((), set r v h)))"
+  [code del]: "update r v = IO (Heap_Monad.heap (\<lambda>h. ((), set_heap r v h)))"
 
 definition modify :: "('a::heap \<Rightarrow> 'a) \<Rightarrow> 'a ref \<Rightarrow> 'a io" where
   "modify f r = do {
@@ -69,6 +69,9 @@ definition modify :: "('a::heap \<Rightarrow> 'a) \<Rightarrow> 'a ref \<Rightar
      r := y;
      return y
    }"
+
+primrec extract_io :: "'a io \<Rightarrow> heap \<Rightarrow> 'a option" where
+  "extract_io (IO v) h = map_option fst (execute v h)"
 
 (* Monadic Combinators *)
 
